Specs/AESGCMKernel.lean
@@ -1,0 +1,175 @@
+/-
+Copyright (c) 2024 Amazon.com, Inc. or its affiliates. All Rights Reserved.
+Released under Apache 2.0 license as described in the file LICENSE.
+Author(s): Yan Peng
+-/
+import Arm.BitVec
+import Specs.AESArm
+import Specs.GCM
+import Specs.AESV8
+import Specs.GCMV8
+
+namespace AESGCMKernel
+
+open BitVec
+
+structure AESGCMLoopVars (in_bytes : Nat) where
+  plaintext : BitVec (in_bytes * 8)
+  input_ptr : Nat -- how many bytes have been processed
+  main_end_input_ptr : Nat -- number of bytes to be processed in main loop
+  Xi : BitVec 128
+  Htable : List (BitVec 128)
+  key : AESV8.AESKey
+
+  ctr0 : BitVec 128
+  ctr1 : BitVec 128
+  ctr2 : BitVec 128
+  ctr3 : BitVec 128
+
+  aes0 : BitVec 128
+  aes1 : BitVec 128
+  aes2 : BitVec 128
+  aes3 : BitVec 128
+
+  ciphertext : BitVec (in_bytes * 8)
+deriving DecidableEq, Repr
+
+set_option diagnostics true
+set_option maxRecDepth 100000
+
+def AESGCMEncKernelLoop {Param : AESArm.KBR} (vars : AESGCMLoopVars in_bytes)
+  : AESGCMLoopVars in_bytes :=
+  if input_ptr ≥ main_end_input_ptr then vars
+  else
+    let bit_len := in_bytes * 8
+    let ctr3 := GCM.inc_s 32 vars.ctr2 (by omega) (by omega)
+    let vars := {vars with ctr3 := ctr3}
+    let H1 := vars.Htable.get! 0
+    let H2 := vars.Htable.get! 2
+    let H3 := vars.Htable.get! 3
+    let H4 := vars.Htable.get! 5
+    let Xi := GCMV8.gcm_ghash_block H4 vars.Xi vars.aes0
+    let Xi := GCMV8.gcm_ghash_block H3 Xi vars.aes1
+    let Xi := GCMV8.gcm_ghash_block H2 Xi vars.aes2
+    let Xi := GCMV8.gcm_ghash_block H1 Xi vars.aes3
+    let start := bit_len - vars.ptr
+    let block0 := extractLsb (start - 1) (start - 128) vars.plaintext
+    let block1 := extractLsb (start - 129) (start - 256) vars.plaintext
+    let block2 := extractLsb (start - 257) (start - 384) vars.plaintext
+    let block3 := extractLsb (start - 385) (start - 512) vars.plaintext
+    let aes0 := block0 ^^^
+      (AESArm.AES_encrypt_with_ks (Param := Param) vars.ctr0 vars.key.rd_key)
+    let aes1 := block1 ^^^
+      (AESArm.AES_encrypt_with_ks (Param := Param) vars.ctr1 vars.key.rd_key)
+    let aes2 := block2 ^^^
+      (AESArm.AES_encrypt_with_ks (Param := Param) vars.ctr2 vars.key.rd_key)
+    let aes3 := block3 ^^^
+      (AESArm.AES_encrypt_with_ks (Param := Param) vars.ctr3 vars.key.rd_key)
+    let ctr0 := GCM.inc_s 32 ctr3 (by omega) (by omega)
+    let ctr1 := GCM.inc_s 32 ctr0 (by omega) (by omega)
+    let ctr2 := GCM.inc_s 32 ctr1 (by omega) (by omega)
+    let ciphertext := BitVec.partInstall (vars.ptr + 127) vars.ptr aes0 vars.ciphertext
+    let ciphertext := BitVec.partInstall (vars.ptr + 255) (vars.ptr + 128) aes1 ciphertext
+    let ciphertext := BitVec.partInstall (vars.ptr + 383) (vars.ptr + 256) aes2 ciphertext
+    let ciphertext := BitVec.partInstall (vars.ptr + 511) (vars.ptr + 384) aes3 ciphertext
+    let vars : AESGCMLoopVars in_bytes :=
+      { plaintext := vars.plaintext,
+        ptr := vars.ptr + 128 * 4,
+        Xi := Xi,
+        Htable := vars.Htable,
+        key := vars.key,
+        ctr0 := ctr0, ctr1 := ctr1,
+        ctr2 := ctr2, ctr3 := vars.ctr3,
+        aes0 := aes0, aes1 := aes1,
+        aes2 := aes2, aes3 := aes3,
+        ciphertext := ciphertext }
+    AESGCMEncKernelLoop (Param := Param) vars
+
+def AESGCMEncKernelHelper {Param : AESArm.KBR}
+  (in_stream : BitVec (in_bytes * 8))
+  (Xi : BitVec 128) (ivec : BitVec 128)
+  (key : AESV8.AESKey) (Htable : List (BitVec 128))
+  : (List (BitVec 8) × BitVec 128) :=
+  let input_ptr := 0
+  -- subtracting 1 from in_bytes because the asssembly wants
+  -- last four blocks be handled in tail code
+  let main_end_input_ptr := input_ptr + ((in_bytes - 1) / 64 * 64)
+  let end_input_ptr := input_ptr + in_bytes
+  if input_ptr ≥ main_end_input_ptr -- if less or equal to 4 blocks
+  then sorry -- tail code
+  else
+    let ciphertext := BitVec.zero (in_bytes * 8)
+
+    have h1 : 128 = Param.block_size := by sorry
+    let ctr0 := BitVec.cast h1 ivec
+    let ctr1 := GCM.inc_s 32 ctr0 (by omega) (by omega)
+    let ctr2 := GCM.inc_s 32 ctr1 (by omega) (by omega)
+    let ctr3 := GCM.inc_s 32 ctr2 (by omega) (by omega)
+
+    let lo := input_ptr * 8
+    let hi := lo + 127
+    have h2 : hi - lo + 1 = 128 := by sorry
+    let block0 := BitVec.cast h2 $ extractLsb 127 0 in_stream
+    let lo := hi + 1
+    let hi := lo + 127
+    let block1 := BitVec.cast h2 $ extractLsb 255 128 in_stream
+    let lo := hi + 1
+    let hi := lo + 127
+    let block2 := BitVec.cast h2 $ extractLsb 383 256 in_stream
+    let lo := hi + 1
+    let hi := lo + 127
+    let block3 := BitVec.cast h2 $ extractLsb 511 384 in_stream
+
+    let aes0 := block0 ^^^ (BitVec.cast h1.symm
+      (AESArm.AES_encrypt_with_ks (Param := Param) ctr0 key.rd_key))
+    let aes1 := block1 ^^^ (BitVec.cast h1.symm
+      (AESArm.AES_encrypt_with_ks (Param := Param) ctr1 key.rd_key))
+    let aes2 := block2 ^^^ (BitVec.cast h1.symm
+      (AESArm.AES_encrypt_with_ks (Param := Param) ctr2 key.rd_key))
+    let aes3 := block3 ^^^ (BitVec.cast h1.symm
+      (AESArm.AES_encrypt_with_ks (Param := Param) ctr3 key.rd_key))
+
+    let ciphertext := BitVec.partInstall 127 0 aes0 ciphertext
+    let ciphertext := BitVec.partInstall 255 128 aes1 ciphertext
+    let ciphertext := BitVec.partInstall 383 256 aes2 ciphertext
+    let ciphertext := BitVec.partInstall 511 384 aes3 ciphertext
+
+    let ctr3 := BitVec.cast h1.symm ctr3
+    let ctr4 := GCM.inc_s 32 ctr3 (by omega) (by omega)
+    let ctr5 := GCM.inc_s 32 ctr4 (by omega) (by omega)
+    let ctr6 := GCM.inc_s 32 ctr5 (by omega) (by omega)
+    -- let ctr7 := GCM.inc_s 32 ctr6 (by omega) (by omega)
+    let vars : AESGCMLoopVars in_bytes :=
+      { plaintext := in_stream,
+        input_ptr := input_ptr + 64,
+        main_end_input_ptr := main_end_input_ptr,
+        Xi := Xi,
+        Htable := Htable,
+        key := key,
+        ctr0 := ctr4, ctr1 := ctr5, ctr2 := ctr6, ctr3 := ctr3,
+        aes0 := aes0, aes1 := aes1, aes2 := aes2, aes3 := aes3,
+        ciphertext := ciphertext }
+    let res := AESGCMEncKernelLoop (Param := Param) vars
+    ( split (BitVec.reverse res.ciphertext) 8 (by omega), res.Xi)
+
+def AESGCMEncKernel (in_blocks : List (BitVec 8))
+  (in_bits : BitVec 64) (Xi : BitVec 128) (ivec : BitVec 128)
+  (key : AESV8.AESKey) (Htable : List (BitVec 128))
+  (h1 : key.rounds = 10#64 ∨ key.rounds = 12#64 ∨ key.rounds = 14#64)
+  (h2: 128 ∣ in_bits.toNat)  -- in_blocks only contains whole blocks
+  (h3: 8 * in_blocks.length = in_bits.toNat)
+  : (List (BitVec 8) × BitVec 128) :=
+  let in_bytes := in_bits.toNat/8
+  have h: 8 * in_blocks.reverse.length = in_bytes * 8 := by
+    simp only [List.length_reverse, h3, in_bytes]; omega
+  let in_stream : BitVec (in_bytes * 8) :=
+    BitVec.cast h $ BitVec.flatten $ List.reverse in_blocks
+  let p := AESV8.KBR_from_AESKey key h1
+  AESGCMEncKernelHelper (Param := p) in_stream Xi ivec key Htable
+
+def AESGCMDecKernel (in_blocks : List (BitVec 8)) (in_bits : BitVec 64)
+  (Xi : BitVec 128) (ivec : BitVec 128) (key : AESKey)
+  (Htable : List (BitVec 128)) : (List (BitVec 8) × BitVec 128) :=
+  sorry
+
+end AESGCMKernel
